Add fsti for dotproduct2

src/examples/GPU.DotProduct2.fst
@@ -15,15 +15,6 @@ module HR = GPU.HReduceU64Plus
 
 #set-options "--z3rlimit 20"
 
-let size : sz = 1024sz
-
-let mul (s1 s2: seq u64)
-  : Ghost (seq u64)
-          (requires Seq.length s1 == Seq.length s2)
-          (ensures fun _ -> True)
-  = Seq.init_ghost (Seq.length s1)
-      (fun i -> U64.mul_mod (Seq.index s1 i) (Seq.index s2 i))
-
 let kpre (nth: nat) (ga1 ga2 r : gpu_array u64 nth) (s1 s2: erased (seq u64))
   (#_: squash ( Seq.length s1 == nth /\ Seq.length s2 == nth )) (tid:nat{tid < nth})
   : slprop =
@@ -36,7 +27,7 @@ let kpost (nth: nat) (ga1 ga2 r : gpu_array u64 nth) (s1 s2: erased (seq u64))
   : slprop =
     ((gpu_pts_to_array #u64 #nth ga1 #(1.0R /. Real.of_int nth) s1 **
     gpu_pts_to_array #u64 #nth ga2 #(1.0R /. Real.of_int nth) s2) **
-    if_ (tid = 0) (HR.gpu_pts_to_slice_sum r 0 nth (mul s1 s2)))
+    if_ (tid = 0) (HR.gpu_pts_to_slice_sum r 0 nth (pmul s1 s2)))
 
 // #set-options "--ext pulse:env_on_err=1"
 
@@ -51,12 +42,12 @@ fn kernel
   requires
     gpu **
     thread_id etid **
-    mbarrier_tok nth (HR.barrier_matrix nth r (mul s1 s2)) 0 (tidx_x etid) **
+    mbarrier_tok nth (HR.barrier_matrix nth r (pmul s1 s2)) 0 (tidx_x etid) **
     kpre nth ga1 ga2 r s1 s2 (thread_index etid)
   ensures
     gpu **
     thread_id etid **
-    (exists* it. mbarrier_tok nth (HR.barrier_matrix nth r (mul s1 s2)) it (tidx_x etid)) **
+    (exists* it. mbarrier_tok nth (HR.barrier_matrix nth r (pmul s1 s2)) it (tidx_x etid)) **
     kpost nth ga1 ga2 r s1 s2 (thread_index etid)
 {
   let tid = thread_idx_x ();
@@ -72,7 +63,7 @@ fn kernel
   (**)fold (gpu_pts_to_array #u64 #nth ga2 #(1.0R /. Real.of_int nth) s2);
   
   let vm = U64.mul_mod v1 v2;
-  (**)let dot_v = hide (mul s1 s2);
+  (**)let dot_v = hide (pmul s1 s2);
   
   (**)unfold (gpu_pts_to_array1 r tid);
   gpu_array_write #u64 #(SZ.v nth) #(SZ.v tid) #(hide (SZ.v tid+1)) r tid vm;
@@ -122,20 +113,20 @@ fn gather_array
 fn main
   (a1 a2: array u64)
   (v1 v2: erased (seq u64))
-  (#_: squash (Seq.length v1 = size /\ Seq.length v2 = size))
+  (#_: squash (Seq.length v1 = dp2_size /\ Seq.length v2 = dp2_size))
   requires cpu ** A.pts_to a1 v1 ** A.pts_to a2 v2
   returns  dp: u64
-  ensures  cpu ** A.pts_to a1 v1 ** A.pts_to a2 v2 ** pure (dp == HR.sum (mul v1 v2))
+  ensures  cpu ** A.pts_to a1 v1 ** A.pts_to a2 v2 ** pure (dp == HR.sum (pmul v1 v2))
 {
-  let ar = A.alloc #u64 0UL size;
+  let ar = A.alloc #u64 0UL dp2_size;
 
-  let ga1 = gpu_array_alloc #u64 size;
-  let ga2 = gpu_array_alloc #u64 size;
+  let ga1 = gpu_array_alloc #u64 dp2_size;
+  let ga2 = gpu_array_alloc #u64 dp2_size;
 
-  GPU.Array.gpu_memcpy_host_to_device a1 ga1 size;
-  GPU.Array.gpu_memcpy_host_to_device a2 ga2 size;
+  GPU.Array.gpu_memcpy_host_to_device a1 ga1 dp2_size;
+  GPU.Array.gpu_memcpy_host_to_device a2 ga2 dp2_size;
   
-  let gr = gpu_array_alloc #u64 size;
+  let gr = gpu_array_alloc #u64 dp2_size;
 
   // Slicing the arrays
   (**)share_array ga1;
@@ -143,60 +134,60 @@ fn main
   (**)gpu_array_slice_1_underspec gr;
 
   // Boring combination of resources
-  (**)bigstar_zip 0 size (shared_array ga1) (shared_array ga2);
-  (**)bigstar_zip 0 size _ (gpu_pts_to_array1 gr);
+  (**)bigstar_zip 0 dp2_size (shared_array ga1) (shared_array ga2);
+  (**)bigstar_zip 0 dp2_size _ (gpu_pts_to_array1 gr);
   (**)rewrite
-    (bigstar 0 size
-      (fun i -> ((shared_array #size ga1 #v1 i **
-                 shared_array #size ga2 #v2 i) **
+    (bigstar 0 dp2_size
+      (fun i -> ((shared_array #dp2_size ga1 #v1 i **
+                 shared_array #dp2_size ga2 #v2 i) **
                  gpu_pts_to_array1 gr i)))
   as
-    (bigstar 0 size (fun i -> kpre size ga1 ga2 gr v1 v2 i))
+    (bigstar 0 dp2_size (fun i -> kpre dp2_size ga1 ga2 gr v1 v2 i))
     by tadmit ();
   (**)bigstar_uneta ();
 
   rewrite
-    bigstar 0 size
-      (kpre size ga1 ga2 gr v1 v2)
+    bigstar 0 dp2_size
+      (kpre dp2_size ga1 ga2 gr v1 v2)
   as
-    bigstar 0 (1 * SZ.v size)
-      (kpre size ga1 ga2 gr v1 v2);
+    bigstar 0 (1 * SZ.v dp2_size)
+      (kpre dp2_size ga1 ga2 gr v1 v2);
 
-  launch_kernel_n_m_barrier #0 1sz size
-    #(kpre size ga1 ga2 gr v1 v2)
-    #(kpost size ga1 ga2 gr v1 v2)
-    #(HR.barrier_matrix size gr (mul v1 v2))
-    (fun etid -> kernel size ga1 ga2 gr #v1 #v2 etid);
+  launch_kernel_n_m_barrier #0 1sz dp2_size
+    #(kpre dp2_size ga1 ga2 gr v1 v2)
+    #(kpost dp2_size ga1 ga2 gr v1 v2)
+    #(HR.barrier_matrix dp2_size gr (pmul v1 v2))
+    (fun etid -> kernel dp2_size ga1 ga2 gr #v1 #v2 etid);
 
   (**)bigstar_eta ();
   // TODO:
   (**)drop_
-        (bigstar 0 (1 * SZ.v size) (fun i -> kpost size ga1 ga2 gr v1 v2 i));
+        (bigstar 0 (1 * SZ.v dp2_size) (fun i -> kpost dp2_size ga1 ga2 gr v1 v2 i));
   (**)assume_
-        (bigstar 0 size
-          (fun i -> ((gpu_pts_to_array #u64 #size ga1 #(1.0R /. Real.of_int size) v1 **
-                    gpu_pts_to_array #u64 #size ga2 #(1.0R /. Real.of_int size) v2) **
-                    if_ (i = 0) (HR.gpu_pts_to_slice_sum gr 0 size (mul v1 v2)))
+        (bigstar 0 dp2_size
+          (fun i -> ((gpu_pts_to_array #u64 #dp2_size ga1 #(1.0R /. Real.of_int dp2_size) v1 **
+                    gpu_pts_to_array #u64 #dp2_size ga2 #(1.0R /. Real.of_int dp2_size) v2) **
+                    if_ (i = 0) (HR.gpu_pts_to_slice_sum gr 0 dp2_size (pmul v1 v2)))
         ));
   
-  (**)bigstar_unzip 0 size _ _;
-  (**)bigstar_unzip 0 size _ _;
+  (**)bigstar_unzip 0 dp2_size _ _;
+  (**)bigstar_unzip 0 dp2_size _ _;
   
-  (**)bigstar_uneta () #0 #0 #size #(shared_array #size ga1 #v1);
+  (**)bigstar_uneta () #0 #0 #dp2_size #(shared_array #dp2_size ga1 #v1);
   gather_array ga1;
-  (**)bigstar_uneta () #0 #0 #size #(shared_array #size ga2 #v2);
+  (**)bigstar_uneta () #0 #0 #dp2_size #(shared_array #dp2_size ga2 #v2);
   gather_array ga2;
 
-  bigstar_if_elim #_ #0 #size 0 (fun _ -> HR.gpu_pts_to_slice_sum #size gr 0 size (mul v1 v2));
+  bigstar_if_elim #_ #0 #dp2_size 0 (fun _ -> HR.gpu_pts_to_slice_sum #dp2_size gr 0 dp2_size (pmul v1 v2));
 
   unfold HR.gpu_pts_to_slice_sum;
   if_elim_true _;
   unfold HR.gpu_pts_to_slice_sum_inner;
-  with res. assert (gpu_pts_to_array_slice gr 0 size res);
-  fold (gpu_pts_to_array #u64 #size gr #1.0R res);
+  with res. assert (gpu_pts_to_array_slice gr 0 dp2_size res);
+  fold (gpu_pts_to_array #u64 #dp2_size gr #1.0R res);
 
   // TODO: don't copy whole array
-  GPU.Array.gpu_memcpy_device_to_host ar gr size;
+  GPU.Array.gpu_memcpy_device_to_host ar gr dp2_size;
 
   gpu_array_free ga1;
   gpu_array_free ga2;
